src/llist.lean
@@ -7,95 +7,84 @@ inductive llist (V : Type) : Type | P : V -> llist | L : V -> llist -> llist
 namespace llist section
     parameters {V W : Type} (adj : V -> V -> Prop)
 
-    def mem : V -> llist V -> Prop | x (P v) := x = v | x (L v l) := x = v ∨ mem x l
-    instance has_mem_llist : has_mem V (llist V) := ⟨mem⟩
+    def fold (f : V -> W) (g : V -> W -> W) : llist V -> W | (P v) := f v | (L v l) := g v (fold l)
 
-    def to_list :             llist V -> list V  |   (P v)    := [v]       |   (L v l)    := v :: to_list l
-    def size    :             llist V -> nat     |   (P _)    := 0         |   (L v l)    := (size l) + 1
-    def head    :             llist V -> V       |   (P v)    := v         |   (L v l)    := v
-    def tail    :             llist V -> list V  |   (P v)    := []        |   (L v l)    := l.head :: tail l
-    def init    :             llist V -> list V  |   (P v)    := []        |   (L v l)    := v :: init l
-    def last    :             llist V -> V       |   (P v)    := v         |   (L v l)    := last l
-    def inside  :             llist V -> list V  |   (P v)    := []        |   (L v l)    := init l
-    def is_path :             llist V -> Prop    |   (P v)    := true      |   (L v l)    := adj v l.head ∧ is_path l
-    def append  :        V -> llist V -> llist V | x (P v)    := L v (P x) | x (L v l)    := L v (append x l)
-    def rev     :             llist V -> llist V |   (P v)    := (P v)     |   (L v l)    := append v (rev l)
-    def nodup   :             llist V -> Prop    |   (P v)    := true      |   (L v l)    := v ∉ l ∧ nodup l
-    def concat  :  llist V -> llist V -> llist V |   (P _) l' := l'        |   (L v l) l' := L v (concat l l')
-    def map     : (V -> W) -> llist V -> llist W | f (P v)    := P (f v)   | f (L v l)    := L (f v) (map f l)
+    def mem (x) : llist V -> Prop | (P v) := x = v | (L v l) := x = v ∨ mem l
+    instance : has_mem V (llist V) := ⟨mem⟩
+
+    @[simp] def to_list          : llist V -> list V  | (P v) := [v]       | (L v l) := v :: to_list l
+    @[simp] def size             : llist V -> nat     | (P _) := 0         | (L v l) := (size l) + 1
+    @[simp] def head             : llist V -> V       | (P v) := v         | (L v l) := v
+    @[simp] def tail             : llist V -> list V  | (P v) := []        | (L v l) := l.head :: tail l
+    @[simp] def init             : llist V -> list V  | (P v) := []        | (L v l) := v :: init l
+    @[simp] def last             : llist V -> V       | (P v) := v         | (L v l) := last l
+    @[simp] def inside           : llist V -> list V  | (P v) := []        | (L v l) := init l
+    @[simp] def is_path          : llist V -> Prop    | (P v) := true      | (L v l) := adj v l.head ∧ is_path l
+    @[simp] def append   (x : V) : llist V -> llist V | (P v) := L v (P x) | (L v l) := L v (append l)
+    @[simp] def rev              : llist V -> llist V | (P v) := (P v)     | (L v l) := append v (rev l)
+    @[simp] def nodup            : llist V -> Prop    | (P v) := true      | (L v l) := v ∉ l ∧ nodup l
+    @[simp] def map (f : V -> W) : llist V -> llist W | (P v) := P (f v)   | (L v l) := L (f v) (map l)
+
+    @[simp] def concat : llist V -> llist V -> llist V | (P _) l' := l' | (L v l) l' := L v (concat l l')
     
-    @[simp] def compat (l₁ l₂ : llist V) := last l₁ = head l₂
-
     variables {x y v w : V} {l l' l'' : llist V}
 
-    @[simp] lemma head_P : head (P v) = v := rfl
+    @[simp] def compat (l l' : llist V) := last l = head l'
 
-    @[simp] lemma last_P : last (P v) = v := rfl
-
-    @[simp] lemma concat_head : compat l l' -> head (concat l l') = head l
-        := llist.cases_on l (λ _ h, eq.trans h.symm rfl) (λ _ _ _, rfl)
+    @[simp] lemma head_concat : compat l l' -> head (concat l l') = head l
+        := by { cases l, exact eq.symm, simp }
 
     @[simp] lemma concat_last : last (concat l l') = last  l'
-        := llist.rec (λ _, rfl) (λ _ _, id) l
+        := by { induction l, refl, simpa }
 
-    @[simp] lemma append_head : head (append v l) = head l
-        := llist.cases_on l (λ _, rfl) (λ _ _, rfl)
+    @[simp] lemma head_append : head (append v l) = head l
+        := by { cases l; refl }
 
-    @[simp] lemma append_last : last (append v l) = v
-        := llist.rec (λ _, rfl) (λ _ _, id) l
+    @[simp] lemma last_append : last (append v l) = v
+        := by { induction l, refl, simpa }
 
     @[simp] lemma rev_append : rev (append v l) = L v (rev l)
-        := by { induction l, refl, rw [append,rev,l_ih], refl }
+        := by { induction l, refl, simp [l_ih] }
 
-    @[simp] lemma rev_head                         : head (rev l)             = last l
-        := by { induction l, refl, rwa [rev,append_head,last] }
+    @[simp] lemma head_rev : head (rev l) = last l
+        := by { induction l, refl, simpa }
 
-    @[simp] lemma rev_last                         : last (rev l)             = head l
-        := by { cases l, refl, rw [rev,append_last,head] }
+    @[simp] lemma last_rev : last (rev l) = head l
+        := by { cases l, refl, simp }
 
-    @[simp] lemma rev_rev                          : rev  (rev l)             = l
-        := by { induction l, refl, rw [rev,rev_append,l_ih] }
+    @[simp] lemma rev_rev : rev (rev l) = l
+        := by { induction l, refl, simpa }
 
-    @[simp] lemma mem_singleton                    : x ∈ P y                <-> x = y
-        := iff.rfl
+    @[simp] lemma mem_singleton : x ∈ P y <-> x = y := iff.rfl
+    @[simp] lemma mem_cons : x ∈ L v l <-> x = v ∨ x ∈ l := iff.rfl
 
-    @[simp] lemma mem_cons                         : x ∈ L v l              <-> x = v ∨ x ∈ l
-        := iff.rfl
+    @[simp] lemma concat_path (h : compat l l') : is_path (concat l l')  <-> is_path l ∧ is_path l'
+        := by { induction l, tauto, simp at h, simp [l_ih h,head_concat h], finish }
 
-    @[simp] lemma concat_path    (h : compat l l') : is_path (concat l l')  <-> is_path l ∧ is_path l'
-        := by { induction l with v v l hr,
-            { tauto },
-            { rw [concat,is_path,hr h,is_path,concat_head], tauto, exact h } }
+    @[simp] lemma mem_append : w ∈ append v l         <-> w = v ∨ w ∈ l
+        := by { induction l, simp, finish, simp [l_ih], finish }
 
-    @[simp] lemma mem_append                       : w ∈ append v l         <-> w = v ∨ w ∈ l
-        := by { induction l, rw [append,mem_cons,mem_singleton,mem_singleton,or_comm],
-            rw [append,mem_cons,l_ih,mem_cons], exact or.left_comm }
+    @[simp] lemma mem_rev : v ∈ rev l <-> v ∈ l
+        := by { induction l, refl, simp [rev], finish }
 
-    @[simp] lemma mem_rev                          : v ∈ rev l              <-> v ∈ l
-        := by { induction l, { rw [rev] }, { rw [rev,mem_append,l_ih,mem_cons] } }
+    @[simp] lemma head_mem : head l ∈ l
+        := by { cases l; simp }
 
-    @[simp] lemma mem_head                         : head l ∈ l
-        := by { cases l, { rw [head,mem_singleton] }, { left, refl } }
+    @[simp] lemma last_mem : last l ∈ l
+        := by { induction l, simp, simp [l_ih] }
 
-    @[simp] lemma mem_last                         : last l ∈ l
-        := by { induction l, { rw [last,mem_singleton] }, { right, assumption } }
+    @[simp] lemma mem_list : x ∈ to_list l <-> x ∈ l
+        := by { induction l, simp, simp [l_ih] }
 
-    @[simp] lemma mem_list                         : x ∈ to_list l          <-> x ∈ l
-        := by { induction l, 
-            { rw [to_list,mem_singleton,list.mem_singleton] }, 
-            { rw [to_list,list.mem_cons_iff,l_ih,mem_cons] } }
-
-    @[simp] lemma append_nodup                     : nodup (append x l)     <-> x ∉ l ∧ nodup l
-        := by { induction l,
-            { rw [append,nodup,nodup,nodup,mem_singleton,mem_singleton], tauto },
-            { rw [append,nodup,l_ih,mem_append,mem_cons,nodup], tauto } }
+    @[simp] lemma nodup_append : nodup (append x l)     <-> x ∉ l ∧ nodup l
+        := by { induction l, simp, finish, simp [l_ih], finish }
 
     @[simp] lemma rev_nodup                        : nodup (rev l)          <-> nodup l
-        := by { induction l, { rw [rev] }, { rw [rev,append_nodup,l_ih,mem_rev,nodup] } }
+        := by { induction l, { rw [rev] }, { rw [rev,nodup_append,l_ih,mem_rev,nodup] } }
 
     @[simp] lemma append_is_path                   : is_path (append v l)   <-> adj (last l) v ∧ is_path l
         := by { induction l, { rw [append,is_path,head,last,is_path,is_path] }, 
-            { rw [append,is_path,l_ih,last,is_path,append_head], tauto } }
+            { rw [append,is_path,l_ih,last,is_path,head_append], tauto } }
 
     @[simp] lemma init_append                      : init (append x l)        = to_list l
         := by { induction l, { refl }, { rw [append,init,l_ih,to_list] } }
@@ -122,7 +111,7 @@ namespace llist section
         := by { cases l, refl, rw [append,inside,init_append,tail,list_head_tail] }
 
     @[simp] lemma tail_append                      : tail (append x l)        = tail l ++ [x]
-        := by { induction l, refl, rw [append,tail,l_ih,append_head,tail], refl }
+        := by { induction l, refl, rw [append,tail,l_ih,head_append,tail], refl }
 
     @[simp] lemma tail_rev                         : tail (rev l)             = list.reverse (init l)
         := by { induction l, refl, rw [rev,tail_append,l_ih,init,list.reverse_cons] }
@@ -131,13 +120,13 @@ namespace llist section
         := by { cases l, refl, rw [rev,inside_append,tail_rev,inside] }
 
     @[simp] lemma rev_is_path  (h : symmetric adj) : is_path (rev l)        <-> is_path l
-        := by { induction l, rw [rev], rw [rev,append_is_path,rev_last,is_path,l_ih], rw symmetric at h, 
+        := by { induction l, rw [rev], rw [rev,append_is_path,last_rev,is_path,l_ih], rw symmetric at h, 
             exact and_congr ⟨@h _ _, @h _ _⟩ iff.rfl }
 
     @[simp] lemma mem_concat     (h : compat l l') : x ∈ concat l l'        <-> x ∈ l ∨ x ∈ l'
         := by { induction l, 
             { rw [concat,mem_singleton], refine ⟨or.inr, _⟩, 
-                intro h1, cases h1, convert mem_head, rwa h1, exact h1 }, 
+                intro h1, cases h1, convert head_mem, rwa h1, exact h1 }, 
             { rw [concat,mem_cons,l_ih h,mem_cons,or.assoc] } }
 
     @[simp] lemma concat_nil      (h : last l = w) : concat l (P w)           = l
@@ -161,7 +150,7 @@ namespace llist section
                     { subst h6, cases h1.2 h7 },
                     { exact h4 x ⟨h6,h7⟩ } },
                 { rintros ⟨⟨h1,h2⟩,h3,h4⟩, rw mem_concat h, push_neg, refine ⟨⟨h1,_⟩,h2,h3,_⟩,
-                    { intro h5, have h6 := h4 v ⟨(or.inl rfl),h5⟩, subst h6, rw <-h at h1, exact (h1 mem_last) },
+                    { intro h5, have h6 := h4 v ⟨(or.inl rfl),h5⟩, subst h6, rw <-h at h1, exact (h1 last_mem) },
                     { rintros x ⟨h5,h6⟩, exact h4 x ⟨(or.inr h5),h6⟩ } } } }
 
     lemma         mem_iff             (h : l = l') : x ∈ l                  <-> x ∈ l'
@@ -187,7 +176,7 @@ namespace llist section
         := by { split,
             { intro, induction l, { right, assumption }, { cases a, { left, left, exact a },
                 cases l_ih a, { left, right, assumption }, { right, rwa last } } },
-            { intro, cases a, exact mem_init a, convert mem_last } }
+            { intro, cases a, exact mem_init a, convert last_mem } }
 
     lemma         mem_head_tail                    : x ∈ l                  <-> x = head l ∨ x ∈ tail l
         := by { cases l, { rw [mem_singleton,head,tail], convert (or_false _).symm },
@@ -212,18 +201,18 @@ namespace llist section
     lemma         nodup_mem_last     (h : nodup l) : last l ∉ init l
         := by { induction l, { rw [init,list.mem_nil_iff], trivial }, 
             { rw [last,init,list.mem_cons_iff], push_neg, split,
-                { intro, apply h.1, convert mem_last, exact a.symm },
+                { intro, apply h.1, convert last_mem, exact a.symm },
                 { exact l_ih h.2 } } }
 
     lemma         rev_compat                       : compat l l' <-> compat l'.rev l.rev
-        := by { rw [compat,compat,rev_last,rev_head,eq_comm] }
+        := by { rw [compat,compat,last_rev,head_rev,eq_comm] }
 
     lemma         concat_append                    : append v (concat l l')  = concat l (append v l')
         := by { induction l; rw [concat,concat], rw [append,l_ih] }
 
     lemma         rev_concat     (h : compat l l') : rev (concat l l')       = concat (rev l') (rev l)
         := by { induction l,
-            { rw [concat,rev,concat_nil], rw [rev_last], exact h.symm },
+            { rw [concat,rev,concat_nil], rw [last_rev], exact h.symm },
             { rw [concat,rev,l_ih h,concat_append,rev] } }
 
     lemma         nodup_init         (h : nodup l) : list.nodup (init l)
@@ -258,7 +247,7 @@ namespace llist section
 end end llist
 
 namespace llist2 section
-    variables {V W : Type} (adj : V -> V -> Prop) {C : llist2 V -> Prop}
+    variables {V W : Type} (f : V -> W) (adj : V -> V -> Prop) {C : llist2 V -> Prop}
 
     @[simp] def cons : V -> llist2 V -> llist2 V | u ⟨x,l⟩ := ⟨u,x::l⟩
 
@@ -270,10 +259,7 @@ namespace llist2 section
 
     def rec'' := @rec' V (λ _, W)
 
-    lemma induction_on (l) (h0 : ∀ x, C ⟨x,[]⟩) (h1 : ∀ {x y ys} (hr : C ⟨y,ys⟩), C ⟨x,y::ys⟩) : C l 
-        := by { apply rec', exact h0, intros, cases l_1, exact h1 a_1 }
-
-    lemma induction_on' (l) (h0 : ∀ x, C ⟨x,[]⟩) (h1 : ∀ (x l) (hr : C l), C (cons x l)) : C l 
+    lemma induction_on (l) (h0 : ∀ x, C ⟨x,[]⟩) (h1 : ∀ (x l) (hr : C l), C (cons x l)) : C l 
         := rec' h0 h1 l
 
     def fold (f : V -> W) (g : V -> W -> W) (l : llist2 V) : W
@@ -312,7 +298,7 @@ namespace llist2 section
     def is_path     : llist2 V -> Prop                 := fold'  (λ _, true)         (λ x, and ∘ adj x)
     def nodup       : llist2 V -> Prop                 := fold'' (λ _, true)         (λ x, and ∘ not ∘ (∈) x)
     
-    def map' (f : V -> W) : llist2 V -> llist2 W := fold (λ x, ⟨f x, []⟩) (cons ∘ f)
+    def map' : llist2 V -> llist2 W := fold (λ x, ⟨f x, []⟩) (cons ∘ f)
 
     def inside  : llist2 V -> list V   | ⟨x,[]⟩ := []     | ⟨x,y::l⟩ := init ⟨y,l⟩
 
@@ -332,15 +318,15 @@ namespace llist2 section
     @[simp] lemma tail_cons    : tail (cons v l)         =  l.head :: l.tail             := by { cases l, refl }
     @[simp] lemma concat'_cons : concat' (cons v l) l'   =  cons v (concat' l l')        := by { cases l, refl }
     @[simp] lemma size'_cons   : size' (cons v l)        =  size' l + 1                  := by { cases l, refl }
+    @[simp] lemma nodup_cons   : nodup (cons v l)       <-> v ∉ l ∧ nodup l              := by { cases l, refl }
+    @[simp] lemma map'_cons    : map' f (cons v l)        =  cons (f v) (map' f l)       := by { cases l, refl }
 
-    @[simp] lemma mem_cons'     : v ∈ llist2.mk x (y::ys) <-> v = x ∨ v ∈ llist2.mk y ys := iff.rfl
-    @[simp] lemma last_cons'    : last ⟨x,y::ys⟩     = last ⟨y,ys⟩               := rfl
-    @[simp] lemma append_cons'  : append w ⟨x,y::ys⟩ = cons x (append w ⟨y,ys⟩)  := rfl
-    @[simp] lemma reverse_cons' : reverse ⟨x,y::ys⟩  = append x (reverse ⟨y,ys⟩) := rfl
-    @[simp] lemma init_cons'    : init ⟨x,y::ys⟩     = x :: init ⟨y,ys⟩          := rfl
-
-    lemma nodup_cons  : nodup (cons v l) <-> v ∉ l ∧ nodup l                        := by { cases l, refl }
-    lemma nodup_cons' : nodup ⟨x,y::ys⟩  <-> x ∉ (⟨y,ys⟩ : llist2 V) ∧ nodup ⟨y,ys⟩ := iff.rfl
+    @[simp] lemma mem_cons'     : v ∈ llist2.mk x (y::ys) <-> v = x ∨ v ∈ llist2.mk y ys             := iff.rfl
+    @[simp] lemma last_cons'    : last ⟨x,y::ys⟩           = last ⟨y,ys⟩                             := rfl
+    @[simp] lemma append_cons'  : append w ⟨x,y::ys⟩       = cons x (append w ⟨y,ys⟩)                := rfl
+    @[simp] lemma reverse_cons' : reverse ⟨x,y::ys⟩        = append x (reverse ⟨y,ys⟩)               := rfl
+    @[simp] lemma init_cons'    : init ⟨x,y::ys⟩           = x :: init ⟨y,ys⟩                        := rfl
+    @[simp] lemma nodup_cons'   : nodup ⟨x,y::ys⟩         <-> x ∉ (⟨y,ys⟩ : llist2 V) ∧ nodup ⟨y,ys⟩ := iff.rfl
 
     @[simp] lemma head_concat : head (concat l l') = head l
         := by { cases l, cases l', refl }
@@ -348,29 +334,34 @@ namespace llist2 section
     @[simp] lemma head_concat' : head (concat' l l') = head l
         := by { rcases l with ⟨x,_|⟨y,ys⟩⟩, refl, simp [concat'] }
 
-    @[simp] lemma last_concat (h : compat l l') : last (concat l l') = last l'
-        := by { revert h, apply induction_on l; intros; cases l' with y l',
-            { cases l' with z l', { exact h }, { simp [concat,last] } },
-            { rw [<-hr h], simp [concat,last] } }
+    @[simp] lemma concat_point : concat' l ⟨x,[]⟩ = l
+        := by { apply induction_on l; intros, refl, simp [hr] }
+
+    lemma concat_point' (h : x = l'.head) : concat' ⟨x,[]⟩ l' = l'
+        := by { cases l', rw [concat',fold_init,h] }
+
+    @[simp] lemma last_concat (h : compat l l') : last (concat' l l') = last l'
+        := by { revert h, apply induction_on l; intros,
+            { rw [concat_point'], exact h },
+            { simp, rw [compat,last_cons] at h, apply hr h } }
 
     @[simp] lemma head_append : head (append v l) = head l
         := by { apply induction_on l; intros, refl, simp }
 
     @[simp] lemma last_append : last (append v l) = v
-        := by { apply induction_on l; intros, refl, rwa [append_cons',last_cons] }
+        := by { apply induction_on l; intros, refl, simpa }
 
     @[simp] lemma rev_append : reverse (append v l) = cons v (reverse l)
-        := by { apply induction_on l; intros, refl, 
-            rw [append_cons',reverse_cons,hr,reverse_cons',append_cons] }
+        := by { apply induction_on l; intros, refl, simp [hr] }
 
     @[simp] lemma rev_head : head (reverse l) = last l
-        := by { apply induction_on l; intros, refl, rw [reverse_cons',head_append,hr], refl }
+        := by { apply induction_on l; intros, refl, simpa }
 
     @[simp] lemma rev_last : last (reverse l) = head l
         := by { apply cases_on' l; intros, refl, rw [reverse_cons,last_append], refl }
 
     @[simp] lemma rev_rev : reverse (reverse l) = l
-        := by { apply induction_on l; intros, refl, rw [reverse_cons',rev_append,hr], refl }
+        := by { apply induction_on l; intros, refl, simp [hr] }
 
     lemma mem_iff : x ∈ l <-> x = head l ∨ x ∈ tail l
         := by { cases l, trivial }
@@ -378,49 +369,47 @@ namespace llist2 section
     @[simp] lemma mem_singleton : x ∈ (⟨y,[]⟩ : llist2 V) <-> x = y
         := by { simp [mem_iff] }
 
-    @[simp] lemma concat_path (h : compat l l') : is_path adj (concat l l') <-> is_path adj l ∧ is_path adj l'
-        := by { revert h, apply induction_on l; intros, 
-            { simp [is_path,concat,last] at h ⊢, subst h, cases l', trivial }, 
-            { cases l', simp [concat,is_path] at hr h ⊢, rw [hr h,and.assoc] } }
+    @[simp] lemma concat_path (h : compat l l') : is_path adj (concat' l l') <-> is_path adj l ∧ is_path adj l'
+        := by { revert h, apply induction_on l; intros,
+            { simp [compat,last] at h, subst h, rw [concat_point'], simp [is_path] },
+            { rw [compat,last_cons] at h, simp [hr h], finish } }
 
     @[simp] lemma mem_append : w ∈ append v l <-> w = v ∨ w ∈ l
-        := by { apply induction_on' l; intros, simp [append,or.comm], 
+        := by { apply induction_on l; intros, simp [append,or.comm], 
             rw [append_cons,mem_cons,mem_cons,hr], finish }
 
     @[simp] lemma mem_rev : v ∈ reverse l <-> v ∈ l
-        := by { apply induction_on l; intros, simp [reverse], 
-            rw [reverse_cons',mem_append,hr,mem_iff,mem_iff], trivial }
+        := by { apply induction_on l; intros, refl, simp [hr] }
 
     @[simp] lemma mem_head : head l ∈ l
         := by { cases l, left, refl }
 
     @[simp] lemma mem_last : last l ∈ l
-        := by { apply induction_on l; intros, { left, refl }, { right, assumption } }
+        := by { apply induction_on l; intros; finish }
 
     @[simp] lemma mem_list : x ∈ to_list l <-> x ∈ l
         := by { cases l, trivial }
 
     @[simp] lemma append_nodup : nodup (append x l) <-> x ∉ l ∧ nodup l
-        := by { apply induction_on' l; intros,
+        := by { apply induction_on l; intros,
             { simp [append,nodup,mem], exact ne_comm },
             { rw [append_cons,nodup_cons,hr,mem_append,nodup_cons], finish } }
 
     @[simp] lemma rev_nodup : nodup (reverse l) <-> nodup l
-        := by { apply induction_on l; intros, { trivial }, 
-            { rw [reverse_cons',append_nodup,hr,mem_rev], trivial } }
+        := by { apply induction_on l; intros, trivial, simp [hr] }
 
     @[simp] lemma append_is_path : is_path adj (append v l) <-> adj (last l) v ∧ is_path adj l
-        := by { apply induction_on' l; intros, { simp [append,is_path,last] }, 
+        := by { apply induction_on l; intros, { simp [append,is_path,last] }, 
             { simp [hr], finish } }
 
     @[simp] lemma init_append : init (append x l) = to_list l
-        := by { apply induction_on' l; intros, refl, { simp [hr] } }
+        := by { apply induction_on l; intros, refl, { simp [hr] } }
 
     @[simp] lemma list_init_last : init l ++ [last l] = to_list l
-        := by { apply induction_on l; intros, refl, rw [init,last,to_list], finish }
+        := by { apply induction_on l; intros, refl, simpa }
 
     @[simp] lemma list_head_init' : v :: inside (cons v l) = init (cons v l)
-        := by { apply induction_on l; intros, refl, simp [cons,inside,init] }
+        := by { apply induction_on l; intros, refl, simp }
 
     @[simp] lemma list_head_init (h : l.tail ≠ []) : head l :: inside l = init l
         := by { revert h, apply cases_on' l; intros, contradiction, refl }
@@ -432,20 +421,19 @@ namespace llist2 section
         := by { cases l with x l, cases l, contradiction, exact list_init_last }
 
     @[simp] lemma init_inside (h : l.tail ≠ []) : init l = (head l) :: inside l
-        := by { revert h, apply induction_on l; intros, contradiction, simp [init,inside] }
+        := by { revert h, apply induction_on l; intros, contradiction, simp }
 
     lemma tail_cons' : tail (cons v l) = to_list l
         := by { apply cases_on' l; intros, refl, simp [to_list] }
 
     @[simp] lemma inside_append : inside (append x l) = tail l
-        := by { apply induction_on' l; intros, refl, simp [tail_cons'] }
+        := by { apply induction_on l; intros, refl, simp [tail_cons'] }
 
     @[simp] lemma tail_append : (append x l).tail = tail l ++ [x]
-        := by { apply induction_on' l; intros, refl, simpa }
+        := by { apply induction_on l; intros, refl, simpa }
 
     @[simp] lemma tail_rev : tail (reverse l) = list.reverse (init l)
-        := by { apply induction_on l; intros, refl, 
-            rw [reverse_cons',init_cons',list.reverse_cons,<-hr,tail_append] }
+        := by { apply induction_on l; intros, refl, simp [hr] }
 
     @[simp] lemma rev_inside : inside (reverse l) = list.reverse (inside l)
         := by { apply cases_on' l; intros, refl, 
@@ -453,8 +441,7 @@ namespace llist2 section
 
     @[simp] lemma rev_is_path (h : symmetric adj) : is_path adj (reverse l) <-> is_path adj l
         := by { apply induction_on l; intros, trivial, 
-            rw [reverse_cons',append_is_path,hr,is_path,rev_last],
-            exact and_congr ⟨@h _ _, @h _ _⟩ iff.rfl }
+            simp [hr], exact and_congr ⟨@h _ _, @h _ _⟩ iff.rfl }
 
     @[simp] lemma mem_concat (h : compat l l') : x ∈ concat l l' <-> x ∈ l ∨ x ∈ l'
         := by { replace h : head l' ∈ l, by { rw compat at h, rw <-h, exact mem_last },
@@ -474,40 +461,40 @@ namespace llist2 section
     lemma concat_assoc : concat (concat l l') l'' = concat l (concat l' l'')
         := by { cases l, cases l', cases l'', simp [concat] }
 
-    lemma concat_nodup (h : compat l l') : nodup (concat l l')
-                <-> nodup l ∧ nodup l' ∧ (∀ v, v ∈ l ∧ v ∈ l' -> v = head l')
-        := by { revert h, apply induction_on l; intros,
-            { simp [compat,last] at h, subst h, rw [concat_nil' rfl], simp [nodup] },
-            { cases l, cases l', simp [concat] at *, rw [nodup_cons', hr h, nodup], clear hr, 
-                simp [mem_iff], push_neg, split,
-                { rintros ⟨⟨h1,h2,h3⟩,h4,h5,h6,h7⟩, refine ⟨⟨⟨h1,h2⟩,h4⟩,h5,_⟩, 
-                    intros v h8 h9, cases h9, assumption,
-                    cases h8, subst h8, contradiction,
-                    cases h8, subst h8, apply h6, exact or.inr h9,
-                    apply h7 v h8, exact or.inr h9 },
-                { rintros ⟨⟨⟨h1,h2⟩,h3⟩,h4,h5⟩, refine ⟨⟨h1,h2,_⟩,h3,h4,_,_⟩,
-                    { intro h7, have h6 := h5 x (or.inl rfl) (or.inr h7), subst h6,
-                        revert h4 h7, cases l'_tail; intros, cases h7, 
-                        simp at h4, apply h4.1, simp at h7, exact h7 },
-                    { exact h5 y (or.inr (or.inl rfl)) },
-                    { intros x, exact h5 x ∘ or.inr ∘ or.inr } } } }
+    -- lemma concat_nodup (h : compat l l') : nodup (concat l l')
+    --             <-> nodup l ∧ nodup l' ∧ (∀ v, v ∈ l ∧ v ∈ l' -> v = head l')
+    --     := by { revert h, apply induction_on l; intros,
+    --         { simp [compat,last] at h, subst h, rw [concat_nil' rfl], simp [nodup] },
+    --         { cases l, cases l', simp [concat] at *, rw [nodup_cons', hr h, nodup], clear hr, 
+    --             simp [mem_iff], push_neg, split,
+    --             { rintros ⟨⟨h1,h2,h3⟩,h4,h5,h6,h7⟩, refine ⟨⟨⟨h1,h2⟩,h4⟩,h5,_⟩, 
+    --                 intros v h8 h9, cases h9, assumption,
+    --                 cases h8, subst h8, contradiction,
+    --                 cases h8, subst h8, apply h6, exact or.inr h9,
+    --                 apply h7 v h8, exact or.inr h9 },
+    --             { rintros ⟨⟨⟨h1,h2⟩,h3⟩,h4,h5⟩, refine ⟨⟨h1,h2,_⟩,h3,h4,_,_⟩,
+    --                 { intro h7, have h6 := h5 x (or.inl rfl) (or.inr h7), subst h6,
+    --                     revert h4 h7, cases l'_tail; intros, cases h7, 
+    --                     simp at h4, apply h4.1, simp at h7, exact h7 },
+    --                 { exact h5 y (or.inr (or.inl rfl)) },
+    --                 { intros x, exact h5 x ∘ or.inr ∘ or.inr } } } }
 
     lemma mem_init (h : x ∈ init l) : x ∈ l
-        := by { revert h, apply induction_on l; intros; cases h, exact or.inl h, exact or.inr (hr h) }
+        := by { revert h, apply induction_on l; intros, cases h,
+            simp at h, simp, cases h, exact or.inl h, exact or.inr (hr h) }
 
     lemma mem_head_init (h : l.tail ≠ []) : head l ∈ init l
         := by { revert h, apply cases_on' l; intros, simp at h, contradiction, left, refl }
 
     lemma mem_last_tail (h : l.tail ≠ []) : last l ∈ tail l
         := by { revert h, apply induction_on l; intros, simp at h, contradiction,
-            cases ys, { left, refl }, { right, rw [last], apply hr, trivial } }
+            simp, revert hr, apply cases_on' l_1; intros, { left, refl }, { right, apply hr, trivial } }
 
     lemma mem_tail : x ∈ tail l -> x ∈ l
         := by { rw mem_iff, exact or.inr }
 
     lemma mem_init_last : x ∈ l <-> x ∈ init l ∨ x = last l
-        := by { apply induction_on l; intros, simp [init,last], 
-            rw [init_cons',list.mem_cons_iff,last_cons',or.assoc,<-hr], trivial }
+        := by { apply induction_on l; intros, simp [init,last], simp [hr], finish }
 
     lemma mem_init_inside' : x ∈ init (cons v l) <-> x = v ∨ x ∈ inside (cons v l)
         := by { cases l, rw [init_cons,cons,inside,list.mem_cons_iff] }
@@ -527,51 +514,42 @@ namespace llist2 section
     lemma nodup_mem_last (h : nodup l) : last l ∉ init l
         := by { revert h, apply induction_on l; intros,
             { simp [last,init] },
-            { rw [last_cons',init_cons',list.mem_cons_iff], push_neg, refine ⟨λ a, _, hr h.2⟩, 
-                apply h.1, convert mem_last, exact a.symm } }
+            { simp at h, simp, push_neg, split, exact λ hh, (hh.symm ▸ h.1) mem_last, exact hr h.2 } }
 
     lemma rev_compat : compat l l' <-> compat l'.reverse l.reverse
         := by { rw [compat,compat,rev_last,rev_head,eq_comm] }
 
     lemma concat_append : append v (concat' l l')  = concat' l (append v l')
-        := by { apply induction_on' l; intros,
+        := by { apply induction_on l; intros,
             { rw [concat',fold_init], apply llist2.ext, rw head_append, simp },
             { simp [hr] } }
 
-    lemma concat_point : concat' l ⟨x,[]⟩ = l
-        := by { apply induction_on' l; intros, refl, simp [hr] }
-
-    lemma concat_point' (h : x = l'.head) : concat' ⟨x,[]⟩ l' = l'
-        := by { cases l', rw [concat',fold_init,h] }
-
     lemma rev_concat (h : compat l l') : reverse (concat' l l') = concat' (reverse l') (reverse l)
-        := by { revert h, apply induction_on' l; intros,
+        := by { revert h, apply induction_on l; intros,
             { simp [last] at h, rw [concat_point' h,reverse,fold_init,concat_point] },
             { simp, rw [hr], rw [concat_append], rw [compat,last_cons] at h, exact h } }
 
     lemma nodup_init (h : nodup l) : list.nodup (init l)
         := by { revert h, apply induction_on l; intros, simp [init],
-            rw [init_cons',list.nodup,list.pairwise_cons], exact ⟨λ u h1 h2, (h2 ▸ h.1) (mem_init h1), hr h.2⟩ }
+            simp at ⊢ h, split, exact h.1 ∘ mem_init, exact hr h.2 }
 
     lemma nodup_of_init : list.nodup (init l) -> last l ∉ init l -> nodup l
-        := by { apply induction_on l; intros, { trivial },
-            { rw [nodup], 
-                rw [init_cons',list.nodup_cons] at a, cases a with h3 h4,
-                rw [last_cons',init_cons',list.mem_cons_iff] at a_1, push_neg at a_1, cases a_1 with h1 h2,
-                refine ⟨_, hr h4 h2⟩,
-                { simp, rw mem_init_last, push_neg, exact ⟨h3, λ h, h1 h.symm⟩ } } }
+        := by { apply induction_on l; intros, trivial,
+            simp at ⊢ a a_1, push_neg at a_1, split,
+                { intro h, cases mem_init_last.mp h, exact a.1 h_1, exact a_1.1 h_1.symm },
+                { exact hr a.2 a_1.2 } }
 
     lemma head_map {f : V -> W} {l : llist2 V} : head (map f l) = f (head l)
         := by { cases l, refl }
 
-    lemma last_map {f : V -> W} {l : llist2 V} : last (map f l) = f (last l)
-        := by { apply induction_on l; intros, refl, simp [map,last], exact hr }
+    lemma last_map {f : V -> W} {l : llist2 V} : last (map' f l) = f (last l)
+        := by { apply induction_on l; intros, refl, simpa }
 
     @[simp] lemma size_append : size' (append v l) = size' l + 1
-        := by { apply induction_on' l; intros, refl, simp [hr] }
+        := by { apply induction_on l; intros, refl, simp [hr] }
 
     lemma size_reverse : size' l.reverse = size' l
-        := by { apply induction_on' l; intros, refl, simpa }
+        := by { apply induction_on l; intros, refl, simpa }
 end end llist2
 
 @[ext] structure llist' (V : Type) (x y : V) := (l : llist V) (hx : l.head = x) (hy : l.last = y)
@@ -596,7 +574,7 @@ namespace llist' section open llist
         := eq.trans l.hy l'.hx.symm
 
     def concat {x y z : V} (l : llist' V x y) (l' : llist' V y z) : llist' V x z
-        := ⟨llist.concat l l', eq.trans (concat_head compat) l.hx, eq.trans concat_last l'.hy⟩
+        := ⟨llist.concat l l', eq.trans (head_concat compat) l.hx, eq.trans concat_last l'.hy⟩
 
     @[simp] lemma concat_P {l : llist' V x y} : concat l (P y) = l
         := by { ext, exact llist.concat_nil l.hy }
@@ -627,8 +605,8 @@ namespace llist2' section open llist2
         := eq.trans l.hy l'.hx.symm
 
     def concat {x y z : V} (l : llist2' V x y) (l' : llist2' V y z) : llist2' V x z
-        := ⟨llist2.concat l l', eq.trans head_concat l.hx, eq.trans (last_concat compat) l'.hy⟩
+        := ⟨llist2.concat' l l', eq.trans head_concat' l.hx, eq.trans (last_concat compat) l'.hy⟩
 
     @[simp] lemma concat_P {l : llist2' V x y} : concat l (P y) = l
-        := by { apply ext, exact concat_nil l.hy }
+        := by { apply ext, apply concat_point }
 end end llist2'
